Split proof into two closed form lemmas
* Remove some of the annoying notation
* Move proof into `Is0.lean`
* State `pseudocompleteness` theorem
* Make proof slightly neater and faster (use `simp only`)

Is0/Programs.lean
@@ -7,14 +7,12 @@ import Mathlib.Tactic.LibrarySearch
 import Mathlib.Tactic.FieldSimp
 
 import Is0.Basic
-import Is0.Ending
 import Is0.Lemmas
 
 namespace Risc0
 
 open MLIRNotation
 
-open MLIRNotation in
 def is0_witness (input : List Felt) : List Felt :=
   let state' :=
     MLIR.run { felts := Map.empty
@@ -43,7 +41,6 @@ def is0_witness (input : List Felt) : List Felt :=
     -- %10 = cirgen.and_eqz %1, %9 : <default>
     -- %11 = cirgen.and_cond %5, %6 : <default>, %10
 
-open MLIRNotation in
 def is0_constraints (input : List Felt) (output : List Felt) : Prop :=
   let state' :=
     MLIR.run { felts := Map.empty
@@ -59,25 +56,17 @@ def is0_constraints (input : List Felt) (output : List Felt) : Prop :=
     "out[0]"    ←ₐ output[0]; -- %3 = cirgen.get %arg1[0] back 0 : <2, mutable>
     "andEqz x"  ←ₐ ⟨"true"⟩ &₀ ⟨"x"⟩; -- %4 = cirgen.and_eqz %1, %2 : <default>
     "if out[0] then eqz x" ←ₐ guard ⟨"out[0]"⟩ & ⟨"true"⟩ with ⟨"andEqz x"⟩;  -- %5 = cirgen.and_cond %1, %3 : <default>, %4
-    "1 - out[0]" ←ₐ ⟨"1"⟩ - ⟨"out[0]"⟩; -- %6 = cirgen.sub %0 : <default>, %3 : <default>
+    "1 - out[0]" ←ₐ Op.Sub ⟨"1"⟩ ⟨"out[0]"⟩; -- %6 = cirgen.sub %0 : <default>, %3 : <default>
     "out[1]"         ←ₐ output[1]; -- %7 = cirgen.get %arg1[1] back 0 : <2, mutable>
-    "x * out[1]"     ←ₐ ⟨"x"⟩ * ⟨"out[1]"⟩; -- %8 = cirgen.mul %2 : <default>, %7 : <default>
-    "x * out[1] - 1" ←ₐ ⟨"x * out[1]"⟩ - ⟨"1"⟩; -- %9 = cirgen.sub %8 : <default>, %0 : <default>
+    "x * out[1]"     ←ₐ Op.Mul ⟨"x"⟩ ⟨"out[1]"⟩; -- %8 = cirgen.mul %2 : <default>, %7 : <default>
+    "x * out[1] - 1" ←ₐ Op.Sub ⟨"x * out[1]"⟩ ⟨"1"⟩; -- %9 = cirgen.sub %8 : <default>, %0 : <default>
     "other cond" ←ₐ ⟨"true"⟩ &₀ ⟨"x * out[1] - 1"⟩; -- %10 = cirgen.and_eqz %1, %9 : <default>
     "if other cond" ←ₐ guard ⟨"1 - out[0]"⟩ & ⟨"if out[0] then eqz x"⟩ with ⟨"other cond"⟩ -- %11 = cirgen.and_cond %5, %6 : <default>, %10
   -- (List.foldr And True) $ List.map (λ e ↦ e = 0) state'.constraints
   (state'.props "if other cond").getD True
 
-open MLIR in
-theorem is0_original_nondet_iff_constraints
-  {input output : List Felt}
-  (h : input.length = 1 ∧ output.length = 2) :
-  (is0_witness input = output ↔ is0_constraints input output) := by
+lemma is0_constraints_closed_form {x y₁ y₂ : Felt} : is0_constraints [x] [y₁, y₂] ↔ (if 1 - y₁ = 0 then if y₁ = 0 then True else x = 0 else (if y₁ = 0 then True else x = 0) ∧ x * y₂ - 1 = 0) := by
   unfold is0_constraints
-  rcases h with ⟨hin, hout⟩
-  rcases input with _ | ⟨x, _ | _⟩ <;> simp at hin ; clear hin
-  rcases output with _ | ⟨y₁, _ | ⟨y₂, ⟨_ | _⟩⟩⟩ <;> simp at hout ; clear hout
-  -- unfold is0_witness
   rw [MLIR.run_Sequence_Assign_collapsible]
   simp only [Op.eval_getInput, List.getD_cons_zero, State.update_val]
   rw [MLIR.run_Sequence_Assign_collapsible]
@@ -132,28 +121,21 @@ theorem is0_original_nondet_iff_constraints
   rw [MLIR.run_assign]
   simp only [Op.eval_andCond, Map.update_get, beq_iff_eq, Option.some.injEq, eq_iff_iff,
   State.update_constraint, Option.getD_some]
-  rw [Map.update_get' (Sub.sub 1 y₁)] <;> try decide
+  rw [Map.update_get' (1 - y₁)] <;> try decide
   swap
-  rw [Map.update_get' (Sub.sub 1 y₁)] <;> try decide
-  rw [Map.update_get' (Sub.sub 1 y₁)] <;> try decide
-  simp
-  rfl
+  rw [Map.update_get' (1 - y₁)] <;> try decide
+  rw [Map.update_get' (1 - y₁)] <;> try decide
+  simp only [Map.update_get, Option.some.injEq]
   rw [Map.update_get' (if y₁ = 0 then True else x = 0)] <;> try decide
-  swap
-  simp
-  simp
-  generalize h :
-    (if Sub.sub 1 y₁ = 0 then
-      if y₁ = 0 then True else x = 0
-        else (if y₁ = 0 then True else x = 0) ∧ HSub.hSub (HMul.hMul x y₂) 1 = 0) = finalCond
+  simp only [Map.update_get]
+
+lemma is0_witness_closed_form {x y₁ y₂ : Felt} : is0_witness [x] = [y₁, y₂] ↔ (if x = 0 then 1 else 0) = y₁ ∧ (if x = 0 then 0 else x⁻¹) = y₂ := by
   unfold is0_witness
   rw [MLIR.run_Sequence_Assign_collapsible]
   simp only [Op.eval_getInput, List.getD_cons_zero, State.update_val]
   rw [MLIR.run_Sequence_Assign_collapsible]
   simp only [Op.eval_isz, Map.update_get, beq_iff_eq, State.update_val]
-  rw [MLIR.run_Sequence_Set_collapsible (if x = 0 then 1 else 0)]
-  swap
-  simp
+  rw [MLIR.run_Sequence_Set_collapsible (if x = 0 then 1 else 0) (by simp only [Map.update_get])]
   simp only
   rw [MLIR.run_Sequence_Assign_collapsible]
   simp only [Op.eval_inv, beq_iff_eq, State.update_val]
@@ -161,44 +143,6 @@ theorem is0_original_nondet_iff_constraints
   simp only
   rw [MLIR.run_set]
   simp only [Map.update_get]
-  apply Iff.intro
-  · intros h₁
-    subst h
-    by_cases eq : x = 0 <;> simp [eq]
-    · by_cases eq₁ : y₁ = 0 <;> simp [eq₁]
-      subst eq₁
-      subst eq
-      simp at h₁
-      simp [List.set] at h₁
-      subst eq
-      simp at h₁
-      simp [List.set] at h₁
-      rcases h₁ with ⟨h₁, h₂⟩
-      subst h₁
-      subst h₂
-      simp
-    · by_cases eq₁ : y₁ = 0 <;> simp [eq₁]
-      · subst eq₁
-        simp [List.set] at h₁
-        rw [←h₁.2]
-        simp [eq]
-      · simp [eq, eq₁, List.set] at h₁
-        tauto
-  -- Other directioon
-  have kekW : x ≠ 0 := sorry
-  subst h
-  intros h
-  simp [kekW]
-  by_cases eq : y₁ = 0 <;> simp [eq] at *
-  · simp at h
-    simp [List.set]
-    field_simp [h]
-    rw [←add_left_inj 1] at h
-    simp at h
-    rw [←h]
-    ring
-  · simp [List.set] at h
-    field_simp [h]
-    simp [List.set]
-    by_cases eq₁ : y₁ = 0 <;> simp [*] at *
+  unfold List.set ; unfold List.set ; simp only [List.cons.injEq, and_true]
+
 end Risc0
