Is0/Is0.lean
@@ -1,13 +1,50 @@
+-- This file contains the MLIR program labeled `ORIGINAL` in the `nonzero-example` output.
 import Mathlib.Data.Nat.Prime
 import Mathlib.Data.Vector
 import Mathlib.Data.ZMod.Defs
 import Mathlib.Data.ZMod.Basic
 import Mathlib.Tactic.LibrarySearch
+import Mathlib.Tactic.FieldSimp
 
 import Is0.Basic
 import Is0.Lemmas
 import Is0.Programs
 
 namespace Risc0
+
+open MLIRNotation
+
+open MLIR in
+theorem is0_constraints_if_is0_witness
+  {input output : List Felt}
+  (h : input.length = 1 ∧ output.length = 2) :
+  (is0_witness input = output → is0_constraints input output) := by
+  rcases h with ⟨hin, hout⟩
+  rcases input with _ | ⟨x, _ | _⟩ <;> simp only [List.length_cons, List.length_singleton, Nat.succ.injEq, add_eq_zero_iff, and_false, OfNat.one_ne_ofNat] at hin ; clear hin
+  rcases output with _ | ⟨y₁, _ | ⟨y₂, ⟨_ | _⟩⟩⟩ <;> simp only [List.length_cons, List.length_singleton, Nat.succ.injEq, add_eq_zero_iff, and_false, OfNat.one_ne_ofNat] at hout ; clear hout
+  rw [is0_constraints_closed_form]
+  rw [is0_witness_closed_form]
+  intros h₁
+  by_cases eq : x = 0 <;> simp only [eq]
+  · by_cases eq₁ : y₁ = 0 <;> simp only [eq₁]
+    subst eq eq₁
+    simp only [ite_true, inv_zero, ite_self] at h₁
+    simp only [List.set, List.cons.injEq, and_true, false_and] at h₁
+    subst eq
+    simp only [ite_true, inv_zero, ite_self] at h₁
+    simp only [List.set, List.cons.injEq, and_true] at h₁
+    rcases h₁ with ⟨h₁, h₂⟩
+    subst h₁ h₂
+    simp only
+  · by_cases eq₁ : y₁ = 0 <;> simp only [eq₁, sub_zero, one_ne_zero, ite_true, true_and, ite_false]
+    · subst eq₁
+      simp only [List.set, List.cons.injEq, ite_eq_right_iff, and_true] at h₁
+      rw [←h₁.2]
+      simp only [eq, ite_false, ne_eq, not_false_iff, mul_inv_cancel, sub_self]
+    · simp only [List.set, eq, ite_false, List.cons.injEq, and_true] at h₁
+      tauto
+
+theorem pseudocompleteness {x y₁ y₂ : Felt} {state : State} :
+  is0_constraints [x] [y₁, y₂] → .Val y₂ = Op.eval {state with felts := Map.empty["x"] := x} (.Isz ⟨"x"⟩) := by sorry
 
 end Risc0
